02_Earleys_Algorithm.thy
@@ -9,7 +9,7 @@ chapter \<open>Earley's Algorithm \label{chapter:2}\<close>
 
 text\<open>
 We present a slightly simplified version of Earley's original recognizer algorithm \cite{Earley:1970},
-omitting Earley's proposed look-ahead since it's primary purpose is to increase the efficiency of the
+omitting Earley's proposed look-ahead since its primary purpose is to increase the efficiency of the
 resulting recognizer. Throughout this thesis we are working with a running example. The considered grammar is a tiny excerpt of a toy
 arithmetic expression grammar: @{term "\<G>"} $::= S \rightarrow \, x \, \vert \, S \rightarrow \, S + S$ and
 the input is @{term \<omega>} $= x + x + x$.
@@ -20,16 +20,16 @@ In detail, the algorithm works as follows: it scans the input @{term \<omega>} $
 $n+1$ Earley bins $B_i$ that are sets of Earley items. An inital bin $B_0$ and one bin $B_{i+1}$ for
 each symbol $a_i$ of the input.
 In general, an Earley item $A \rightarrow \, \alpha \bullet \beta, i, j$ consists of four parts: a production rule of the grammar that we are currently
-scanning, a bullet signalling how much of the production's right-hand side we have recognized so far,
-an origin $i$ describing the position of @{term \<omega>} where we started scanning, and an end $j$ indicating
-the position  of @{term \<omega>} we are currently considering next for the remaining right-hand side of the production rule.
+considering, a bullet signalling how much of the production's right-hand side we have recognized so far,
+an origin $i$ describing the position in @{term \<omega>} where we started scanning, and an end $j$ indicating
+the position in @{term \<omega>} we are currently considering next for the remaining right-hand side of the production rule.
 Note that there will be only one set of earley items or only one bin $B$ and we say an item is conceptually part of bin $B_j$ if it's end is the index $j$.
 Table \ref{tab:earley_bins} lists the items for our example grammar. Bin $B_4$ contains for example the item $S \rightarrow \, S + \bullet S, 2, 4$.
-Or, we are scanning the rule $S \rightarrow \, S + S$, have recognized the substring from $2$ to $4$ (the first index being
+Or, we are considering the rule $S \rightarrow \, S + S$, have recognized the substring from $2$ to $4$ (the first index being
 inclusive the second one exclusive) of @{term \<omega>} by $\alpha = S +$, and are trying to scan $\beta = S$ from position 4 in \omega. 
 
 The algorithm initializes $B$ by applying the \textit{Init} operation. It then proceeds to execute
-the \textit{Scan}, \textit{Predict} and \textit{Complete} operations listed in figure \ref{fig:inference_rules}
+the \textit{Scan}, \textit{Predict} and \textit{Complete} operations listed in Figure \ref{fig:inference_rules}
 until there are no more new items being generated and added to $B$. Next we describe these four operations
 in detail:
 
@@ -38,14 +38,14 @@ in detail:
     $S \rightarrow \, \bullet\alpha, 0, 0$ for each production rule containing the start symbol $S$ on its left-hand side.
 
     For our example \textit{Init} adds the items $S \rightarrow \, \bullet x, 0, 0$ and $S \rightarrow \, \bullet S + S, 0 , 0$.
-  \item The \textit{Scan} operation applies if there is a terminal to the right side of the bullet, or items of the form $A \rightarrow \, \alpha \bullet a \beta, i, j$,
+  \item The \textit{Scan} operation applies if there is a terminal to the right-hand side of the bullet, or items of the form $A \rightarrow \, \alpha \bullet a \beta, i, j$,
     and the $j$-th symbol of @{term \<omega>} matches the terminal symbol following the bullet. We add one new item $A \rightarrow \, \alpha a \bullet \beta, i, j+1$
     to $B$ moving the bullet over the scanned terminal symbol.
 
     Considering our example, bin $B_3$ contains
-    the item $S \rightarrow \, S \bullet + S, 2, 3$, the third element of @{term \<omega>} is the terminal $+$, so we add the
+    the item $S \rightarrow \, S \bullet + S, 2, 3$, the third symbol of @{term \<omega>} is the terminal $+$, so we add the
     item $S \rightarrow \, S + \bullet S, 2, 4$ to the conceptual bin $B_4$.
-  \item The \textit{Predict} operation is applicable to an item when there is a non-terminal to the right of
+  \item The \textit{Predict} operation is applicable to an item when there is a non-terminal to the right-hand side of
     the bullet or items of the form $A \rightarrow \, \alpha \bullet B \beta, i, j$. It adds one new item $B \rightarrow \, \bullet \gamma, j, j$
     to the bin for each alternate $B \rightarrow \, \gamma$ of that non-terminal.
 
@@ -55,7 +55,7 @@ in detail:
     rule, the origin and end are set to $j = 2$ to indicate that we are starting to scan in the current bin and
     have not scanned anything so far.
   \item The \textit{Complete} operation applies if we process an item with the bullet at the end of the
-    right side of its production rule. For an item $B \rightarrow \, \gamma \bullet, j, k$ we have successfully scanned the substring
+    right-hand side of its production rule. For an item $B \rightarrow \, \gamma \bullet, j, k$ we have successfully scanned the substring
     \omega[j..k) and are now going back to the origin bin $B_j$ where we predicted this non-terminal. There we look for any item of the form
     $A \rightarrow \, \alpha \bullet B \beta, i, j$ containing a bullet in front of the non-terminal we completed, or the reason we
     predicted it on the first place. Since we scanned the predicted non-terminal successfully, we are allowed to
@@ -63,9 +63,9 @@ in detail:
     the origin and end indices.
 
     Looking back at our example, we can add the item $S \rightarrow \, S + S \bullet, 0, 5$
-    for two different reasons corresponding conceptually to the two different ways we can derive \omega.
+    for two different reasons corresponding to the two different ways we can derive \omega.
     When processing $S \rightarrow \, x \bullet, 4, 5$ we find $S \rightarrow \, S + \bullet S, 0, 4$ in the origin
-    bin $B_4$ which corresponds to recognizing $(x + x) + x$. We 'add' the same item again
+    bin $B_4$ which corresponds to recognizing $(x + x) + x$. We would add the same item again
     while applying the \textit{Complete} operation to $S \rightarrow \, S + S \bullet, 2, 5$ and $S \rightarrow \, S + \bullet S, 0, 2$
     which corresponds to recognizing the input as $x + (x + x)$.
 \end{enumerate}
@@ -84,11 +84,11 @@ $$S \rightarrow \, \alpha \bullet, 0, @{term "length \<omega> + 1"} \in B \,\,\,
 It follows from the following three lemmas:
 
 \begin{enumerate}
-  \item Termination: there only exist a finite number of Earley items
   \item Soundness: for every generated item there exists an according derivation: \\
      $A \rightarrow \, \alpha \bullet \beta, i, j \in B \,\,\, \textrm{implies} \,\,\, A \, \xRightarrow{\ast} \, @{term \<omega>}[i..j) \beta$
   \item Completeness: for every derivation we generate an according item: \\
      $A \, \xRightarrow{\ast} \, @{term \<omega>}[i..j) \beta \,\,\, \textrm{implies} \,\,\, A \rightarrow \, \alpha \bullet \beta, i, j \in B$
+  \item Finiteness: there only exist a finite number of Earley items
 \end{enumerate}
 \<close>
 
@@ -102,11 +102,11 @@ text\<open>
       {$S \rightarrow \, \bullet\alpha, 0, 0$}
   
       \inferrule [Scan]
-      {$A \rightarrow \, \alpha \bullet a \beta, i, j$ \\ $@{term \<omega>}[j] = a$}
+      {$A \rightarrow \, \alpha \bullet a \beta, i, j$ \\ $@{term "\<omega>"}[j] = a$}
       {$A \rightarrow \, \alpha a \bullet \beta, i, j+1$}
   
       \inferrule [Predict]
-      {$A \rightarrow \, \alpha \bullet B \beta, i, j$ \\ $B \rightarrow \, \gamma \, \in \, @{term "\<G>"}$}
+      {$A \rightarrow \, \alpha \bullet B \beta, i, j$ \\ $(B \rightarrow \, \gamma) \, \in \, @{term "\<G>"}$}
       {$B \rightarrow \, \bullet \gamma, j, j$}
   
       \inferrule [Complete]
